secure_api/box/Box.PKAE.fst
@@ -8,6 +8,7 @@ open FStar.HyperStack.ST
 open FStar.Endianness
 
 open Box.Plain
+open Box.Index
 
 module AE = Box.AE
 module ODH = Box.ODH
@@ -21,9 +22,13 @@ assume val random_bytes: n:nat -> lbytes n
 //
 //assume val pkae_flag: bool
 
+let n32 = n:nat{n <= 32}
+let bytes32 = b:bytes{Seq.length b <= 32}
+
 val ae_enc_star: n:(n:nat{AE_Spec.valid_plain_length n}) -> b:lbytes (n+16){AE_Spec.valid_cipher_length (n+16)}
 let ae_enc_star n = Seq.append (random_bytes n) (random_bytes 16)
 
+val pp : pp:plain_package{pp.flag == Flags.pkae}
 let pp = PP Flags.pkae AE_Spec.valid_plain_length AE_Spec.valid_cipher_length (fun n -> n = AE_Spec.noncelen)
 
 // For some reason it doesn't verify if there is an additional refinement on the output of secretbox_open_easy
@@ -49,193 +54,272 @@ let hsalsa20_hash input = H.hsalsa20 input zero_nonce
 
 let odh_params = ODH.OP (ODH_Spec.serialized_point_length) (ODH_Spec.scalar_length) (H.keylen) (ODH_Spec.base_point) (ODH_Spec.scalarmult) (hsalsa20_hash)
 
+
+noeq type public_key_encryption_scheme (public_key_length:n32) (secret_key_length:n32) =
+  | PKES:
+    gen: (unit -> lbytes secret_key_length*lbytes public_key_length) ->
+    enc: (p:plain pp -> n:nonce pp -> pk:lbytes public_key_length -> sk:lbytes secret_key_length -> c:cipher pp) ->
+    enc_star: (plain_length:nat{pp.valid_plain_length plain_length} -> c:cipher pp) ->
+    dec: (c:cipher pp -> n:nonce pp -> pk:lbytes public_key_length -> sk:lbytes secret_key_length -> option (p:plain pp)) ->
+//    correctness: (p:bytes -> k:lbytes key_length -> n:lbytes nonce_length -> Lemma
+//    (requires True)
+//    (ensures (
+//      let dec_result = dec (enc p k n) k n in
+//      Some? dec_result
+//      /\ Some?.v dec_result == p
+//    ))
+      //    ) ->
+    public_key_encryption_scheme public_key_length secret_key_length
+
+let cryptobox :public_key_encryption_scheme (PKAE_Spec.dh_keylen) (PKAE_Spec.dh_keylen) = PKES (fun () -> random_bytes 32,random_bytes 32) PKAE_Spec.cryptobox (ae_enc_star) PKAE_Spec.cryptobox_open
+
+noeq type pkae_parameters =
+  | PK_Param:
+  public_key_length: n32 ->
+  secret_key_length: n32 ->
+  pke_scheme: public_key_encryption_scheme public_key_length secret_key_length ->
+  pkae_parameters
+
+val pkp: pkae_parameters
+let pkp = PK_Param odh_params.ODH.share_length odh_params.ODH.exponent_length cryptobox
+
+let pkae_index_package = ip:index_package{
+  Leaf_IP? ip
+  /\ (match ip with
+    | Leaf_IP t rgn log -> t == lbytes pkp.public_key_length)
+  /\ id ip == lbytes pkp.public_key_length
+  }
+
+val pkey : Type0
+let pkey = ODH.share odh_params
+//val get_pkey_id: (#pp:plain_package) -> (#pkp:pkae_parameters pp) -> (#ip:index_package pkp) -> pk:pkey pkp -> Tot (i:id ip)
+
 #set-options "--z3rlimit 300 --max_ifuel 1 --max_fuel 0"
-noeq abstract type pkae_package (#pp:plain_package) (#pkp:pkae_parameters pp) (ip:index_package pkp) =
+val get_pkey_raw: pkey -> Tot (lbytes pkp.public_key_length)
+let get_pkey_raw = ODH.get_share_raw
+
+val skey : Type0
+let skey = ODH.exponent odh_params
+val get_skey_raw: skey -> GTot (lbytes pkp.secret_key_length)
+let get_skey_raw = ODH.get_exponent_raw
+val get_pkey_raw_from_skey_raw: lbytes pkp.secret_key_length -> lbytes pkp.public_key_length
+let get_pkey_raw_from_skey_raw skey_raw = odh_params.ODH.exponentiate skey_raw odh_params.ODH.generator
+val get_pkey_from_skey: sk:skey -> pk:pkey{get_pkey_raw pk = get_pkey_raw_from_skey_raw (get_skey_raw sk)}
+let get_pkey_from_skey = ODH.get_exp_share
+
+let compatible_keys (sk:skey) (pk:pkey) = get_pkey_raw pk <> get_pkey_raw (get_pkey_from_skey sk)
+
+#set-options "--z3rlimit 30 --max_ifuel 2 --max_fuel 2"
+let compose_ip (ip:pkae_index_package) : ip':index_package{
+  ip' == Node_IP [ip;ip]
+  /\ id ip == lbytes pkp.public_key_length
+  /\ id ip' == id ip * id ip
+  /\ id ip' == lbytes pkp.public_key_length * lbytes pkp.public_key_length
+} =
+  let ip' = Node_IP [ip;ip] in
+  assert(unfold_id [ip;ip] == id ip * id ip);
+  assert(unfold_id [ip;ip] == id ip');
+  ip'
+
+let composed_id (ip:pkae_index_package) (pk1:pkey) (pk2:pkey{
+    get_pkey_raw pk1 <> get_pkey_raw pk2
+  }) : (id (compose_ip ip)) =
+  let pk1_raw = get_pkey_raw pk1 in
+  let pk2_raw = get_pkey_raw pk2 in
+  let le_sh1 = little_endian pk1_raw in
+  let le_sh2 = little_endian pk2_raw in
+  assert(hasEq (lbytes pkp.secret_key_length * lbytes pkp.public_key_length));
+  if le_sh1 < le_sh2 then
+    pk1_raw,pk2_raw
+  else
+    pk2_raw,pk1_raw
+
+val pkae_package: (ip:pkae_index_package) -> Type u#1
+#set-options "--z3rlimit 30 --max_ifuel 0 --max_fuel 0"
+noeq abstract type pkae_package (ip:pkae_index_package) =
   | PKAE_P :
     pkae_rgn:erid ->
-    kp: Key.key_package ip AE_Spec.keylen (AE.key AE_Spec.keylen) ->
-    op: ODH.odh_package #ip #AE_Spec.keylen #(AE.key AE_Spec.keylen) kp odh_params ->
-    ap: AE.ae_package kp ae_params ->
-    pkae_package
+    kp: Key.key_package (compose_ip ip){kp.Key.key_length = odh_params.ODH.hash_length} ->
+    op: ODH.odh_package #odh_params ip kp ->
+    ap: AE.ae_package #pp (compose_ip ip) ae_params ->
+    pkae_package ip
 
-#set-options "--z3rlimit 300 --max_ifuel 1 --max_fuel 0"
-let create_pkae_package rgn pp =
+#set-options "--z3rlimit 90 --max_ifuel 1 --max_fuel 1"
+val create_pkae_package: (ip:pkae_index_package) -> rgn:erid -> ST (pkae_package ip)
+  (requires (fun h0 -> True))
+  (ensures (fun h0 pkae_p h1 ->
+    modifies (Set.singleton rgn) h0 h1
+  ))
+let create_pkae_package ip rgn =
   let pkae_rgn = new_region rgn in
-  let ip = create_index_package pkae_rgn in
-  //let pp = PP Flags.pkae AE_Spec.valid_plain_length in
-  let kp = AE.create_ae_key_package ip AE_Spec.keylen in
-  let op = ODH.create_odh_package pkae_rgn kp odh_params in
-  let ap = AE.create_ae_package pkae_rgn kp ae_params in
-  PKAE_P pkae_rgn ip kp op ap
+  let kp = AE.create_ae_key_package (compose_ip ip) AE_Spec.keylen in
+  let op = ODH.create_odh_package ip pkae_rgn kp in
+  let ap = AE.create_ae_package #(compose_ip ip) #pp pkae_rgn ae_params in
+  PKAE_P pkae_rgn kp op ap
 
-let pkey = ODH.share odh_params
-let get_pkey_raw = ODH.get_share_raw
-let get_pkey_id pk = PK_id (ODH.get_share_raw pk)
+#set-options "--z3rlimit 90 --max_ifuel 1 --max_fuel 1"
+val gen_footprint: (#ip:pkae_index_package) -> pkae_package ip -> h0:mem -> h1:mem -> Type0
+let gen_footprint #ip pkae_p h0 h1 = ODH.gen_dh_footprint #odh_params ip h0 h1
 
-let skey = ODH.exponent odh_params
-let get_skey_raw = ODH.get_exponent_raw
-let get_pkey_raw_from_skey_raw skey_raw = odh_params.ODH.exponentiate skey_raw odh_params.ODH.generator
-let get_pkey_from_skey = ODH.get_exp_share
-let get_skey_id sk = get_pkey_id (ODH.get_exp_share sk)
+#set-options "--z3rlimit 90 --max_ifuel 1 --max_fuel 1"
+val gen : (#ip:pkae_index_package) -> pkae_p:pkae_package ip -> ST (keypair:(skey*pkey))
+  (requires (fun h0 ->
+    Flags.model
+  ))
+  (ensures (fun h0 (sk,pk) h1 ->
+    get_pkey_from_skey sk == pk
+    /\ honest #ip (get_pkey_raw pk)
+    /\ registered #ip (get_pkey_raw pk)
+    /\ gen_footprint pkae_p h0 h1
+  ))
+let gen #ip pkae_p = ODH.gen_dh #odh_params ip
 
-//let nonce = AE.nonce ae_params
-//let ciphertext = AE.ciphertext ae_params
+val coerce_pkey_footprint: (#ip:pkae_index_package) -> pkae_p:pkae_package ip -> pk_raw:lbytes pkp.public_key_length -> h0:mem -> h1:mem -> Type0
+let coerce_pkey_footprint #ip pkae_p pk_raw h0 h1 = ODH.coerce_dh_sh_footprint #odh_params ip pk_raw h0 h1
 
-let get_index_package #pp pkae_p = pkae_p.ip
-
-let gen_footprint #pp pkae_p h0 h1 = ODH.gen_dh_footprint pkae_p.ip odh_params h0 h1
-
-let gen #pp pkae_p = ODH.gen_dh pkae_p.ip odh_params
-
-let coerce_pkey_footprint #pp pkae_p pk_raw h0 h1 = ODH.coerce_dh_sh_footprint pkae_p.ip odh_params pk_raw h0 h1
-
-let coerce_pkey #pp pkae_p pk_raw =
-  let pk = ODH.coerce_dh_sh pkae_p.ip odh_params pk_raw in
+val coerce_pkey : (#ip:pkae_index_package) -> pkae_p:pkae_package ip -> pk_raw:lbytes pkp.public_key_length -> ST (pk:pkey)
+  (requires (fun h0 ->
+    corrupt #ip pk_raw
+    /\ registered #ip pk_raw
+  ))
+  (ensures (fun h0 pk h1 ->
+    get_pkey_raw pk = pk_raw
+    /\ coerce_pkey_footprint pkae_p pk_raw h0 h1
+  ))
+let coerce_pkey #ip pkae_p pk_raw =
+  let pk = ODH.coerce_dh_sh ip  pk_raw in
   pk
 
-let coerce_skey_footprint #pp pkae_p sk_raw h0 h1 = ODH.coerce_dh_exp_footprint pkae_p.ip odh_params sk_raw h0 h1
+val coerce_skey_footprint: (#ip:pkae_index_package) -> pkae_p:pkae_package ip -> sk_raw:lbytes pkp.secret_key_length -> h0:mem -> h1:mem -> Type0
+let coerce_skey_footprint #ip pkae_p sk_raw h0 h1 = ODH.coerce_dh_exp_footprint #odh_params ip sk_raw h0 h1
 
-let coerce_skey #pp pkae_p sk_raw =
-  let sk = ODH.coerce_dh_exp pkae_p.ip odh_params sk_raw in
+val coerce_skey : (#ip:pkae_index_package) -> pkae_p:pkae_package ip -> sk_raw:lbytes pkp.secret_key_length -> ST (sk:skey)
+  (requires (fun h0 ->
+    let pk_raw = get_pkey_raw_from_skey_raw sk_raw in
+    corrupt #ip pk_raw
+    /\ registered #ip pk_raw
+  ))
+  (ensures (fun h0 sk h1 ->
+    let pk_raw = get_pkey_raw_from_skey_raw sk_raw in
+    get_skey_raw sk = sk_raw
+    /\ coerce_skey_footprint pkae_p sk_raw h0 h1
+  ))
+let coerce_skey #ip pkae_p sk_raw =
+  let sk = ODH.coerce_dh_exp #odh_params ip sk_raw in
   sk
 
-let compose_ids pk1 pk2 = compose_id (pk1) pk2
-
-//let compatible_keys pk sk = get_pkey_from_skey sk <> pk
-
-//#set-options "--z3rlimit 5 --max_ifuel 0 --max_fuel 0"
-//val create_key : pkae_p:pkae_package -> i:inst_id -> message_log_value i
-//let create_key pkae_p i =
-//  //assert(protected_plain pp i == AE.message_log_value pp i);
-//  //assert(protected_plain pp i == message_log_value i);
-//  let (ae_value : AE.message_log_value pp i) = coerce pkae_p.ip i (AE.zero_bytes (fun n -> true) 5) in
-//  admit()
-//  //let pkae_value : message_log_value i = ae_value in
-//  //pkae_value
-
-let get_log_rgn #pp pkae_p = AE.get_log_rgn pkae_p.ap
+val get_log_rgn: (#ip:pkae_index_package) -> (pkae_p:pkae_package ip) -> Tot (rgn:erid)
+let get_log_rgn #ip pkae_p = AE.get_log_rgn pkae_p.ap
 
 // We need an explicit ciphertext type with valid_length predicate.
 //val get_pp: pkae_p:pkae_package -> pp:plain_package{pp.flag == Flags.pkae /\ pp.valid_length}
 //let get_pp #pp pkae_p = AE.get_ap_pp pkae_p.ap
 
-#set-options "--z3rlimit 300 --max_ifuel 1 --max_fuel 0"
-//val get_log: pkae_p:pkae_package -> GTot (AE.ae_message_log ae_params (AE.get_ap_pp pkae_p.ap) (AE.get_log_rgn pkae_p.ap))
-//val get_log: pkae_p:pkae_package -> GTot (AE.ae_message_log ae_params (AE.get_ap_pp pkae_p.ap) (AE.get_log_rgn pkae_p.ap))
-let get_log #pp pkae_p =
-  assert(ae_params.AE.scheme.AE.pp == pp);
-  admit()
-  //AE.get_ap_log #pkae_p.ip #_ #_ #ae_params pkae_p.ap
+#set-options "--z3rlimit 150 --max_ifuel 0 --max_fuel 0"
+val get_log: (#ip:pkae_index_package) -> (pkae_p:pkae_package ip) -> GTot (Mem.message_log (compose_ip ip) pp (get_log_rgn pkae_p))
+let get_log #ip pkae_p =
+  let ap :AE.ae_package #pp (compose_ip ip) ae_params = pkae_p.ap in
+  let rgn :erid = AE.get_log_rgn pkae_p.ap in
+  let rgn' :erid = get_log_rgn pkae_p in
+  assert(rgn' == rgn);
+  let log : Mem.message_log (compose_ip ip) pp rgn = AE.get_ap_log #(compose_ip ip) #pp #ae_params ap in
+  log
 
-let encrypt_footprint pkae_p pk sk n c p h0 h1 =
+let nonce_is_unique (#ip:pkae_index_package) (pkae_p:pkae_package ip) i n h0 =
+  Flags.model ==>
+    (let log: Mem.i_message_log (compose_ip ip) pp (get_log_rgn pkae_p) = get_log pkae_p in
+    forall c . MM.fresh log (i,n,c) h0)
+
+#set-options "--z3rlimit 30 --max_ifuel 8 --max_fuel 8"
+let extended_message_log
+  (#ip:pkae_index_package)
+  (pkae_p:pkae_package ip)
+  (pk:pkey)
+  (sk:skey{compatible_keys sk pk})
+  (n:nonce pp)
+  (c:cipher pp)
+  (p:protected_plain #(compose_ip ip) pp (composed_id ip pk (get_pkey_from_skey sk)))
+  (h0:mem) (h1:mem) =
+  let i : id (compose_ip ip) = composed_id ip pk (get_pkey_from_skey sk) in
+  let log_value: protected_plain #(compose_ip ip) pp i = p in
+  //if Flags.model then
+  //  let log_key: id (compose_ip ip)*nonce pp*cipher pp  = i,n,c in
+  //  let log: Mem.i_message_log (compose_ip ip) pp (get_log_rgn pkae_p) = get_log pkae_p in
+  //  //sel h1 log == MM.upd (sel h0 log) log_key p
+  //           True
+  //  /\ witnessed (MM.defined log log_key)
+  //  ///\ witnessed (MM.contains log log_key p)
+  //else
+    True
+
+#set-options "--z3rlimit 30 --max_ifuel 2 --max_fuel 2"
+val encrypt_footprint:
+  (#ip:pkae_index_package) ->
+  (pkae_p:pkae_package ip) ->
+  (pk:pkey) ->
+  (sk:skey{compatible_keys sk pk}) ->
+  (n:nonce pp) ->
+  (c:cipher pp) ->
+  (p:protected_plain #(compose_ip ip) pp (composed_id ip pk (get_pkey_from_skey sk))) ->
+  (h0:mem) ->
+  (h1:mem) ->
+  Type0
+
+let encrypt_footprint #ip pkae_p pk sk n c p h0 h1 =
   ODH.dh_op_memory_footprint pkae_p.op pk sk h0 h1
-  /\ AE.encrypt_footprint pkae_p.ap h0 h1
+  /\ AE.encrypt_footprint #(compose_ip ip) pkae_p.ap h0 h1
 
-let decrypt_footprint pkae_p pk sk n c p h0 h1 =
+let decrypt_footprint #ip pkae_p pk sk n c p h0 h1 =
   ODH.dh_op_memory_footprint pkae_p.op pk sk h0 h1
   /\ AE.decrypt_footprint pkae_p.ap h0 h1
 
-let enc_spec pkae_p p pk sk n = PKAE_Spec.cryptobox p n pk sk
+//let enc_spec pkae_p p pk sk n = PKAE_Spec.cryptobox p n pk sk
+//
+//// Maybe require function to get cipher length from plain_length
+//let enc_star pkae_p plain_length = random_bytes (plain_length+16)
+//
+//val dec_spec: pkae_p:pkae_package -> c:ciphertext -> pk:lbytes pkey_length -> sk:lbytes skey_length -> n:nonce -> option (p:plain (get_pp pkae_p))
 
-// Maybe require function to get cipher length from plain_length
-let enc_star pkae_p plain_length = random_bytes (plain_length+16)
+//#set-options "--z3rlimit 100 --max_ifuel 1 --max_fuel 0"
+//let dec_spec pkae_p c pk sk n =
+//  let option_p:option (plain pkae_p.pp) = PKAE_Spec.cryptobox_open c n pk sk in
+//  assert(pkae_p.pp == get_pp pkae_p);
+//  match option_p with
+//  | Some (p:plain (pkae_p.pp)) ->
+//    let (p:plain (get_pp pkae_p)) = p in
+//    admit()
+//    //Some p
+//  | None -> None
+//  //let option_pp:option (plain (get_pp pkae_p)) = option_p in
+//  //admit()
 
-val dec_spec: pkae_p:pkae_package -> c:ciphertext -> pk:lbytes pkey_length -> sk:lbytes skey_length -> n:nonce -> option (p:plain (get_pp pkae_p))
-
-#set-options "--z3rlimit 100 --max_ifuel 1 --max_fuel 0"
-let dec_spec pkae_p c pk sk n =
-  let option_p:option (plain pkae_p.pp) = PKAE_Spec.cryptobox_open c n pk sk in
-  assert(pkae_p.pp == get_pp pkae_p);
-  match option_p with
-  | Some (p:plain (pkae_p.pp)) ->
-    let (p:plain (get_pp pkae_p)) = p in
-    admit()
-    //Some p
-  | None -> None
-  //let option_pp:option (plain (get_pp pkae_p)) = option_p in
-  //admit()
-
-#set-options "--z3rlimit 300 --max_ifuel 0 --max_fuel 0"
-val encrypt: pkae_package:pkae_package -> pk:pkey -> sk:skey{ODH.get_share_raw pk <> ODH.get_share_raw (ODH.get_exp_share sk)} -> n:nonce -> p:protected_plain pp (ODH.create_id pk (ODH.get_exp_share sk)) -> ST ciphertext
+#set-options "--z3rlimit 30 --max_ifuel 2 --max_fuel 2"
+val encrypt:
+  #ip:pkae_index_package ->
+  pkae_p:pkae_package ip ->
+  pk:pkey ->
+  sk:skey{compatible_keys sk pk} ->
+  n:nonce pp ->
+  p:protected_plain #(compose_ip ip) pp (composed_id pk (get_pkey_from_skey sk)) ->
+  ST (cipher pp)
   (requires (fun h0 ->
-    let i = ODH.create_id pk (ODH.get_exp_share sk) in
-    match sel h0 pkae_package.ap_log i with
-    | Some ap ->
-      contains h0 (AE.get_ap_log ap)
-      /\ AE.nonce_is_unique ap n h0
-    | None -> True
+    let i = composed_id pk (get_pkey_from_skey sk) in
+    nonce_is_unique pkae_p i n h0
+    /\ registered #(compose_ip ip) i
   ))
   (ensures (fun h0 c h1 ->
-    let i = ODH.create_id pk (ODH.get_exp_share sk) in
-    let both_honest = ODH.exp_hon sk && ODH.sh_hon pk in
-    let kp_log = ODH.get_op_log pkae_package.op in
-    // Describe ap_log state
-    Some? (sel h1 pkae_package.ap_log i)
-    /\ (let ap = Some?.v (sel h1 pkae_package.ap_log i) in
-    (if Some? (sel h0 pkae_package.ap_log i) then
-      sel h1 pkae_package.ap_log == sel h0 pkae_package.ap_log
-      /\ sel h1 (AE.get_ap_log ap) == MM.upd (sel h0 (AE.get_ap_log ap)) (n,c) p
-    else
-      sel h1 pkae_package.ap_log == MM.upd (sel h0 pkae_package.ap_log) i ap
-      /\ (forall n' . n' =!= n ==> AE.nonce_is_unique ap n' h1))
-    // Describe modified memory regions
-    /\ (let modified_regions_ap_op = Set.union
-        (AE.encrypt_modified_regions ap)
-        (ODH.dh_op_modified_regions pkae_package.op pk sk h0)
-      in
-      let modified_regions_extend_ap_log = Set.union (Set.singleton pkae_package.ap_rgn) (Set.singleton pkae_package.ap_log_rgn) in
-      let modified_regions =
-        if Some? (sel h0 pkae_package.ap_log i) then
-          modified_regions_ap_op
-        else
-          Set.union modified_regions_ap_op modified_regions_extend_ap_log
-      in
-      modifies modified_regions h0 h1)
-    /\ ODH.dh_op_log_change pkae_package.op pk sk h0 h1
-    // Describe functionality
-    /\ (let k =
-        if both_honest && ODH.get_flag() then
-          Some?.v (MM.sel (sel h1 (ODH.get_op_log pkae_package.op)) i)
-        else
-          ODH.(odh_params.hash (odh_params.exponentiate (ODH.get_exponent_raw sk) (ODH.get_share_raw pk)))
-      in
-      ODH.dh_op_functional_spec pkae_package.op pk sk k h1
-    )
-    /\ ((both_honest /\ ODH.get_flag()) ==>
-        (let k = Some?.v (MM.sel (sel h1 (ODH.get_op_log pkae_package.op)) i) in
-        AE.encrypt_functional_spec ap k n c p)
-      )
-      // In case we have a dishonest key or we don't idealize, we can't guarantee anything.
-    )
+    let i = composed_id pk (get_pkey_from_skey sk) in
+    encrypt_footprint #ip pkae_p pk sk n c p h0 h1
+    /\ ((honest #(compose_ip ip) i /\ Flags.pkae) ==>
+      c == pkp.pke_scheme.enc_star (Plain.length p))
+    /\ ((corrupt #(compose_ip ip) i \/ ~(Flags.pkae)) ==>
+      c == pkp.pke_scheme.enc (Plain.repr #(compose_ip ip) #pp  p) n (get_pkey_raw pk) (get_skey_raw sk))
+    /\ extended_message_log #ip pkae_p i n c p h0 h1
   ))
 
-#set-options "--z3rlimit 300 --max_ifuel 0 --max_fuel 0"
-let encrypt pkae_package pk sk n p =
-  let i = ODH.create_id pk (ODH.get_exp_share sk) in
-  recall pkae_package.ap_log;
-  let k = ODH.dh_op pkae_package.op pk sk in
-  let h1 = get() in
-  ODH.recall_op_log pkae_package.op;
-  let ap =
-    match get_ap_from_log pkae_package i with
-    | Some ap ->
-      ap
-    | None ->
-      let ap = AE.create_ae_package pkae_package.ap_rgn kp ae_params pp in
-      MM.extend pkae_package.ap_log i ap;
-      ap
-  in
-  let c = AE.encrypt ap k n p in
-  //assert(
-  //    let both_honest = ODH.exp_hon sk && ODH.sh_hon pk in
-  //    (both_honest /\ ODH.get_flag()) ==>
-  //      (let k' = Some?.v (MM.sel (sel h1 (ODH.get_op_log pkae_package.op)) i) in
-  //      AE.encrypt_functional_spec ap k n c p
-  //      )
-  //    );
-  //    admit();
-  //assert(AE.encrypt_functional_spec ap k n c p);
-  c
+#set-options "--z3rlimit 30 --max_ifuel 0 --max_fuel 0"
+let encrypt #ip pkae_p pk sk n p =
+  admit()
 
 val decrypt: pkae_package:pkae_package -> pk:pkey -> sk:skey{ODH.get_share_raw pk <> ODH.get_share_raw (ODH.get_exp_share sk)} -> n:nonce -> c:ciphertext -> ST (option (p:protected_plain pp (ODH.create_id pk (ODH.get_exp_share sk))))
   (requires (fun h0 ->
