secure_api/box/Box.Key.fst
@@ -22,12 +22,14 @@ noeq type key_package (ip:index_package) =
 val create_key_package:
   (#ip:index_package) ->
   (flag:Type0) ->
-  (key_length:(n:nat{n<=32})) ->
+  (param_key_length:(n:nat{n<=32})) ->
   (key_type:(id ip -> Type0)) ->
-  (param_getGT: (#i:id ip -> k:key_type i -> GTot (lbytes key_length))) ->
-  (param_leak: (#i:id ip{corrupt i \/ ~flag} -> k:key_type i -> (raw:lbytes key_length{raw = param_getGT k}))) ->
+  (param_getGT: (#i:id ip -> k:key_type i -> GTot (lbytes param_key_length))) ->
+  (param_leak: (#i:id ip{corrupt i \/ ~flag} -> k:key_type i -> (raw:lbytes param_key_length{raw = param_getGT k}))) ->
   (param_gen: (i:id ip -> k:key_type i)) ->
-  (param_coerce: (i:id ip{corrupt i \/ ~flag} -> raw:lbytes key_length -> (k:key_type i{raw = param_getGT k}))) ->
-  (kp:key_package ip)
+  (param_coerce: (i:id ip{corrupt i \/ ~flag} -> raw:lbytes param_key_length -> (k:key_type i{raw = param_getGT k}))) ->
+  (kp:key_package ip{
+    kp.key_length == param_key_length
+  })
 let create_key_package #ip flag key_length key_type getGT leak gen coerce =
   KP flag key_length key_type getGT leak gen coerce
